a "clean" interface with write_cbor

src/cbor/CBOR.SteelST.fst
@@ -3,70 +3,12 @@ open Steel.ST.OnRange
 open Steel.ST.GenElim
 
 module Cbor = CBOR.SteelST.Raw
-module U64 = FStar.UInt64
-module U8 = FStar.UInt8
-module SZ = FStar.SizeT
 module LPA = LowParse.SteelST.ArrayPtr.IntroElim
 module LPS = LowParse.SteelST.SeqMatch
-module R = Steel.ST.Reference
-module A = Steel.ST.Array
 module LW = LowParse.SteelST.L2ROutput.IntroElim
 
-noeq
-type cbor_int = {
-  typ: Cbor.major_type_uint64_or_neg_int64;
-  value: U64.t;
-}
-
-noeq
-type cbor_string = {
-  typ: Cbor.major_type_byte_string_or_text_string;
-  byte_length: U64.t;
-  payload: A.array U8.t;
-  permission: perm;
-}
-
-noeq
-type cbor_serialized = {
-  byte_size: SZ.t;
-  payload: LPS.byte_array;
-  footprint: LPA.array LPS.byte; // ghost
-}
-
-noeq
-type cbor_tagged = {
-  tag: U64.t;
-  payload: R.ref cbor;
-  footprint: Ghost.erased cbor;
-}
-
-and cbor_array = {
-  count: U64.t;
-  payload: A.array cbor;
-  footprint: Ghost.erased (Seq.seq cbor);
-}
-
-and cbor_map_entry = {
-  key: cbor;
-  value: cbor;
-}
-
-and cbor_map = {
-  entry_count: U64.t;
-  payload: A.array cbor_map_entry;
-  footprint: Ghost.erased (Seq.seq cbor_map_entry);
-}
-
-and cbor =
-| CBOR_Case_Int64 of cbor_int
-| CBOR_Case_String of cbor_string
-| CBOR_Case_Tagged of cbor_tagged
-| CBOR_Case_Array of cbor_array
-| CBOR_Case_Map of cbor_map
-| CBOR_Case_Simple_value of Cbor.simple_value
-| CBOR_Case_Serialized of cbor_serialized
-
-let dummy_cbor : cbor = CBOR_Case_Simple_value 0uy
+let cbor_serialized_payload_t = LPS.byte_array
+let cbor_serialized_footprint_t = LPA.array LPS.byte
 
 let raw_data_item_match_serialized_prop
   (c: cbor)
@@ -2067,54 +2009,6 @@ let serialize_cbor_nonempty
 : Lemma
   (Seq.length (serialize_cbor c) > 0)
 = ()
-
-noextract
-let write_cbor_postcond
-  (va: Cbor.raw_data_item)
-  (out: A.array U8.t)
-  (vout': Seq.seq U8.t)
-  (res: SZ.t)
-: Tot prop
-= let s = serialize_cbor va in
-  Seq.length vout' == A.length out /\
-  (res = 0sz <==> Seq.length s > Seq.length vout') /\
-  (res <> 0sz ==> (
-    SZ.v res == Seq.length s /\
-    Seq.slice vout' 0 (Seq.length s) `Seq.equal` s
-  ))
-
-[@@__reduce__]
-let write_cbor_post
-  (va: Ghost.erased Cbor.raw_data_item)
-  (c: cbor)
-  (vout: Ghost.erased (Seq.seq U8.t))
-  (out: A.array U8.t)
-  (res: SZ.t)
-  (vout': Seq.seq U8.t)
-: Tot vprop
-= 
-  A.pts_to out full_perm vout' `star`
-  pure (write_cbor_postcond va out vout' res)
-
-inline_for_extraction
-noextract
-let steel_ifthenelse
-  (cond: bool)
-  (#pre: vprop)
-  (#ret_t: Type)
-  (#post: ret_t -> vprop)
-  (body_true: (squash (cond == true)) ->
-    STT ret_t
-    (pre)
-    (fun v -> post v)
-  )
-  (body_false: (squash (cond == false)) ->
-    STT ret_t
-    (pre)
-    (fun v -> post v)
-  )
-: STF ret_t pre post True (fun _ -> True)
-= if cond then body_true () else body_false ()
 
 let write_cbor
   (#va: Ghost.erased Cbor.raw_data_item)
