src/cbor/CBOR.SteelST.fsti
@@ -1,0 +1,139 @@
+module CBOR.SteelST
+open Steel.ST.Util
+
+module Cbor = CBOR.Spec.Type
+module U64 = FStar.UInt64
+module U8 = FStar.UInt8
+module SZ = FStar.SizeT
+module R = Steel.ST.Reference
+module A = Steel.ST.Array
+
+noeq
+type cbor_int = {
+  typ: Cbor.major_type_uint64_or_neg_int64;
+  value: U64.t;
+}
+
+noeq
+type cbor_string = {
+  typ: Cbor.major_type_byte_string_or_text_string;
+  byte_length: U64.t;
+  payload: A.array U8.t;
+  permission: perm;
+}
+
+inline_for_extraction
+noextract
+val cbor_serialized_payload_t: Type0
+
+[@@erasable]
+val cbor_serialized_footprint_t: Type0
+
+noeq
+type cbor_serialized = {
+  byte_size: SZ.t;
+  payload: cbor_serialized_payload_t;
+  footprint: cbor_serialized_footprint_t;
+}
+
+noeq
+type cbor_tagged = {
+  tag: U64.t;
+  payload: R.ref cbor;
+  footprint: Ghost.erased cbor;
+}
+
+and cbor_array = {
+  count: U64.t;
+  payload: A.array cbor;
+  footprint: Ghost.erased (Seq.seq cbor);
+}
+
+and cbor_map_entry = {
+  key: cbor;
+  value: cbor;
+}
+
+and cbor_map = {
+  entry_count: U64.t;
+  payload: A.array cbor_map_entry;
+  footprint: Ghost.erased (Seq.seq cbor_map_entry);
+}
+
+and cbor =
+| CBOR_Case_Int64 of cbor_int
+| CBOR_Case_String of cbor_string
+| CBOR_Case_Tagged of cbor_tagged
+| CBOR_Case_Array of cbor_array
+| CBOR_Case_Map of cbor_map
+| CBOR_Case_Simple_value of Cbor.simple_value
+| CBOR_Case_Serialized of cbor_serialized
+
+inline_for_extraction
+noextract
+let dummy_cbor : cbor = CBOR_Case_Simple_value 0uy
+
+val raw_data_item_match
+  (c: cbor)
+  (v: Cbor.raw_data_item)
+: Tot vprop
+
+val serialize_cbor
+  (c: Cbor.raw_data_item)
+: GTot (Seq.seq U8.t)
+
+val serialize_cbor_inj
+  (c1 c2: Cbor.raw_data_item)
+: Lemma
+  (requires (serialize_cbor c1 == serialize_cbor c2))
+  (ensures (c1 == c2))
+
+val serialize_cbor_nonempty
+  (c: Cbor.raw_data_item)
+: Lemma
+  (Seq.length (serialize_cbor c) > 0)
+
+noextract
+let write_cbor_postcond
+  (va: Cbor.raw_data_item)
+  (out: A.array U8.t)
+  (vout': Seq.seq U8.t)
+  (res: SZ.t)
+: Tot prop
+= let s = serialize_cbor va in
+  Seq.length vout' == A.length out /\
+  (res = 0sz <==> Seq.length s > Seq.length vout') /\
+  (res <> 0sz ==> (
+    SZ.v res == Seq.length s /\
+    Seq.slice vout' 0 (Seq.length s) `Seq.equal` s
+  ))
+
+[@@__reduce__]
+let write_cbor_post
+  (va: Ghost.erased Cbor.raw_data_item)
+  (c: cbor)
+  (vout: Ghost.erased (Seq.seq U8.t))
+  (out: A.array U8.t)
+  (res: SZ.t)
+  (vout': Seq.seq U8.t)
+: Tot vprop
+= 
+  A.pts_to out full_perm vout' `star`
+  pure (write_cbor_postcond va out vout' res)
+
+val write_cbor
+  (#va: Ghost.erased Cbor.raw_data_item)
+  (c: cbor)
+  (#vout: Ghost.erased (Seq.seq U8.t))
+  (out: A.array U8.t)
+  (sz: SZ.t)
+: ST SZ.t
+    (raw_data_item_match c (Ghost.reveal va) `star`
+      A.pts_to out full_perm vout
+    )
+    (fun res -> 
+      raw_data_item_match c (Ghost.reveal va) `star`
+      exists_ (write_cbor_post va c vout out res)
+    )
+    (SZ.v sz == A.length out)
+    (fun _ -> True)
